Some useful free_var proofs

coq/theories/functional/FunEnv.v
@@ -6,11 +6,12 @@ Module Type FunEnvT.
   Parameter env : Type.
   Parameter empty : env.
   Parameter lookup : env -> name -> option Value.
-  Parameter insert : name * Value -> env -> env.
+  Parameter insert_some : name * Value -> env -> env.
+  Parameter insert : name * option Value -> env -> env.
   Parameter remove : name -> env -> env.
 
   Axiom lookup_insert_eq : forall v x n,
-      lookup (insert (x, n) v) x = Some n.
+      lookup (insert (x, n) v) x = n.
 
   Axiom lookup_insert_neq : forall v x1 x2 n,
       x1 <> x2 ->
@@ -19,11 +20,18 @@ Module Type FunEnvT.
   Axiom insert_insert_eq : forall v x n1 n2,
       insert (x, n1) (insert (x, n2) v) = insert (x, n1) v.
 
+  Axiom insert_insert_neq : forall v x1 x2 n1 n2,
+      x1 <> x2 ->
+      insert (x1, n1) (insert (x2, n2) v) = insert (x2, n2) (insert (x1, n1) v).
+
   Axiom insert_remove : forall v x n,
       insert (x, n) (remove x v) = insert (x, n) v.
 
   Axiom lookup_empty : forall x,
       lookup empty x = None.
+
+  Axiom insert_lookup_self : forall n env,
+    insert (n, lookup env n) env = env.
 
 End FunEnvT.
 
@@ -31,13 +39,15 @@ Module FunEnv : FunEnvT.
   Definition env := name -> option Value.
   Definition empty : env := fun _ => None.
   Definition lookup (v : env) (x : name) : option Value := v x.
-  Definition insert (p : name * Value) (v : env) : env :=
+  Definition insert_some (p : name * Value) (v : env) : env :=
     fun x => if x =? fst p then Some (snd p) else v x.
+  Definition insert (p : name * option Value) (v : env) : env :=
+    fun x => if x =? fst p then (snd p) else v x.
   Definition remove (x : name) (v : env) : env :=
     fun y => if x =? y then None else v y.
 
   Theorem lookup_insert_eq : forall v x n,
-      lookup (insert (x, n) v) x = Some n.
+      lookup (insert (x, n) v) x = n.
   Proof.
     intros; unfold lookup, insert, fst; rewrite Nat.eqb_refl; reflexivity.
   Qed.
@@ -58,6 +68,16 @@ Module FunEnv : FunEnvT.
     unfold insert; destruct (_ =? _); reflexivity.
   Qed.
 
+  Theorem insert_insert_neq : forall v x1 x2 n1 n2,
+      x1 <> x2 ->
+      insert (x1, n1) (insert (x2, n2) v) = insert (x2, n2) (insert (x1, n1) v).
+  Proof.
+    intros; apply functional_extensionality; intros.
+    unfold insert; destruct (_ =? _) eqn:?; destruct (x =? fst (x2, n2)) eqn:?; try reflexivity.
+    rewrite Nat.eqb_eq in *; unfold fst in *; subst.
+    contradiction.
+  Qed.
+
   Theorem insert_remove : forall v x n,
       insert (x, n) (remove x v) = insert (x, n) v.
   Proof.
@@ -69,4 +89,13 @@ Module FunEnv : FunEnvT.
   Theorem lookup_empty : forall x,
       lookup empty x = None.
   Proof. reflexivity. Qed.
+
+  Theorem insert_lookup_self : forall n env,
+    insert (n, lookup env n) env = env.
+  Proof.
+    intros; apply functional_extensionality; intros.
+    unfold insert, lookup, fst; destruct (_ =? _) eqn:?; [|reflexivity].
+    unfold snd; rewrite Nat.eqb_eq in Heqb; unfold fst in Heqb; subst.
+    reflexivity.
+  Qed.
 End FunEnv.
